progress steal

theories/code.v
@@ -38,6 +38,7 @@ Section code.
       "array" +ₗ "b" <- "v" ;;
       bot "deque" <- "b" + #1.
   
+(* TODO: change return value to (bool, val) so that we can push and pop #() *)
   Definition pop : val :=
     λ: "deque",
       let: "array" := arr "deque" in
@@ -78,15 +79,58 @@ Definition dequeΣ : gFunctors :=
 Global Instance subG_dequeΣ {Σ} : subG dequeΣ Σ → dequeG Σ.
 Proof. solve_inG. Qed.
 
+(* TODO: move this to helpers.v *)
+Section Inbound.
+  Definition deque_bound (t b : nat) (l : list val) :=
+    t ≤ b /\ b < length l /\ length l = CAP_CONST.
+
+  Lemma deque_bound_init : deque_bound 0 0 (replicate (Z.to_nat CAP_CONST) #0).
+  Proof.
+    unfold deque_bound. repeat split; auto.
+    rewrite replicate_length. replace (Z.to_nat CAP_CONST) with 10 by auto. lia.
+  Qed.
+
+  Lemma deque_bound_2_length t1 b1 t2 b2 l1 l2 :
+    deque_bound t1 b1 l1 → deque_bound t2 b2 l2 → length l1 = length l2.
+  Admitted.
+
+  Lemma deque_bound_insert t b l i v :
+    deque_bound t b l → i < length l → deque_bound t b (<[b:=v]> l).
+  Admitted.
+
+  Lemma deque_bound_extend_right t b l :
+    deque_bound t b l → b < length l → deque_bound t (S b) l.
+  Admitted.
+
+  Lemma deque_bound_shrink_left t b l : 
+    deque_bound t b l → t < b → deque_bound (S t) b l.
+  Admitted.
+End Inbound.
+
 Section RA.
   Context `{!heapGS Σ, !dequeG Σ} (N : namespace).
   Notation iProp := (iProp Σ).
 
+  (* TODO [URGENT]: we actually need mono_list of [0..t), not just mono_nat of t *)
   Definition mono_toparr (γt : gname) (t : nat) (l : list val) : iProp :=
     let tl := match l with | [] => (2*t) | _ => (2*t+1) end in
     mono_nat_auth_own γt 1 tl.
 
-  Lemma mono_toparr_append (l1 l2 : list val) (γt : gname) (t : nat) :
+  Definition mono_toparr_lb (γt : gname) (t : nat) (l : list val) : iProp :=
+    let tl := match l with | [] => (2*t) | _ => (2*t+1) end in
+    mono_nat_lb_own γt tl.
+
+  Lemma mono_toparr_get_lb (γt : gname) (t : nat) (l : list val) :
+    mono_toparr γt t l ==∗ mono_toparr γt t l ∗ mono_toparr_lb γt t l.
+  Proof.
+  Admitted.
+
+  Lemma mono_toparr_lb_own_top (γt : gname) (t1 t2 : nat) (l1 l2 : list val) :
+    mono_toparr γt t1 l1 -∗ mono_toparr_lb γt t2 l2 -∗ ⌜t2 ≤ t1⌝.
+  Proof.
+  Admitted.
+
+  Lemma mono_toparr_append (γt : gname) (l1 l2 : list val) (t : nat) :
     mono_toparr γt t l1 ==∗ mono_toparr γt t (l1 ++ l2).
   Proof.
     iIntros "mta". destruct l2. { rewrite app_nil_r. auto. }
@@ -94,6 +138,11 @@ Section RA.
     unfold mono_toparr. simpl.
     iMod (mono_nat_own_update (t+(t+0)+1) with "mta") as "[mta _]"; auto. lia.
   Qed.
+
+  Lemma mono_toparr_top (γt : gname) (t1 t2 : nat) (l1 l2 : list val) :
+    t1 ≤ t2 →
+    mono_toparr γt t1 l1 ==∗ mono_toparr γt t2 l2.
+  Admitted.
 End RA.
 
 Section proof.
@@ -109,8 +158,7 @@ Section proof.
       top ↦ #t ∗ bot ↦{#1/2} #b ∗ arr ↦∗{#1/2} l ∗
       ghost_var γq (1/2) (slice l t b) ∗
       mono_toparr γt t (slice l t b) ∗
-      ⌜t ≤ b⌝ ∗
-      ⌜length l = CAP_CONST⌝.
+      ⌜deque_bound t b l⌝.
 
   Definition is_deque (γq γt : gname) (q : val) : iProp :=
     ∃ (arr top bot : loc),
@@ -135,6 +183,9 @@ Section proof.
     by iApply "IH".
   Qed.
 
+  Ltac autoall :=
+    auto; try by (unfold deque_bound in *; unfold CAP_CONST in *; lia).
+
   Lemma new_deque_spec :
     {{{ True }}}
       new_deque #()
@@ -142,20 +193,19 @@ Section proof.
       is_deque γq γt q ∗ deque_content γq [] ∗
       own_deque γq q
     }}}.
-  Proof.
+  Proof with autoall.
     iIntros (Φ) "_ HΦ".
-    wp_lam. wp_alloc arr as "[arr↦1 arr↦2]". { unfold CAP_CONST. lia. }
+    wp_lam. wp_alloc arr as "[arr↦1 arr↦2]"...
     wp_pures. wp_alloc b as "[b↦1 b↦2]". wp_alloc t as "t↦".
     iMod (ghost_var_alloc []) as (γq) "[γ1 γ2]".
     iMod (mono_nat_own_alloc 0) as (γt) "[γt _]".
     iMod (inv_alloc dequeN _ (deque_inv γq γt arr t b)
       with "[t↦ b↦1 arr↦1 γ1 γt]") as "Inv".
-    { iNext. iExists 0, 0, _. iFrame "t↦ b↦1 arr↦1". by iFrame. }
-    wp_pures. iModIntro. iApply "HΦ".
-    iSplit; auto.
-    - iExists _, _, _. auto.
-    - iSplitR "b↦2 arr↦2"; auto.
-      iExists _,_,_,0,_. iFrame. auto.
+    { iNext. iExists 0, 0, _. iFrame "t↦ b↦1 arr↦1". iFrame.
+      iPureIntro. apply deque_bound_init. }
+    wp_pures. iModIntro. iApply "HΦ". iSplit.
+    - iExists _, _, _...
+    - iSplitR "b↦2 arr↦2"... iExists _,_,_,0,_. iFrame...
   Qed.
 
   Lemma push_spec γq γt q (v : val) :
@@ -164,7 +214,7 @@ Section proof.
     <<< ∀∀ l : list val, deque_content γq l >>>
       push q v @ ↑N
     <<< deque_content γq (l ++ [v]) ∗ own_deque γq q, RET #() >>>.
-  Proof with auto; try lia.
+  Proof with autoall.
     iIntros "#Is Own" (Φ) "AU".
       iDestruct "Own" as (arr top bot b l) "(-> & %HL & b👑 & arr👑)".
       iDestruct "Is" as (arr' top' bot') "[%Is Inv]".
@@ -173,44 +223,42 @@ Section proof.
 
     (* load bot *)
     wp_bind (! _)%E.
-    iInv "Inv" as (t1 b1 l1) ">(t↦ & b↦ & arr↦ & γ & mta & [%Htb1 %HL1])".
+    iInv "Inv" as (t1 b1 l1) ">(t↦ & b↦ & arr↦ & γ & mta & %BOUND1)".
       iDestruct (mapsto_agree with "b↦ b👑") as "%".
         injection H as [=]. apply Nat2Z.inj in H.
-      iDestruct (array_agree with "arr↦ arr👑") as "%"...
-      subst. clear HL.
+      iDestruct (array_agree with "arr↦ arr👑") as "%"... subst.
     wp_load.
     
     iModIntro. iSplitL "t↦ b↦ arr↦ γ mta".
       { iExists _,_,_. iFrame "t↦ b↦ arr↦ γ"... }
-    wp_pures. case_bool_decide.
-      { wp_pures. iApply loop_spec... iNext. iIntros... }
-    assert (b < CAP_CONST)... rename H0 into BOUND. clear H.
+    wp_pures. case_bool_decide as HbC.
+      { wp_pures. iApply loop_spec... }
     wp_pures.
 
     (* store value *)
     wp_bind (_ <- _)%E.
-    iInv "Inv" as (t2 b2 l2) ">(t↦ & b↦ & arr↦ & γ & mta & [%Htb2 %HL2])".
+    iInv "Inv" as (t2 b2 l2) ">(t↦ & b↦ & arr↦ & γ & mta & %BOUND2)".
       iDestruct (mapsto_agree with "b↦ b👑") as "%".
         injection H as [=]. apply Nat2Z.inj in H.
       iDestruct (array_agree with "arr↦ arr👑") as "%"...
-      subst. clear t1 Htb1 HL1.
+      subst. clear t1 BOUND1.
     iCombine "arr↦ arr👑" as "arr↦".
-    iApply (wp_store_offset with "arr↦").
-      { rewrite lookup_lt_is_Some... }
+    iApply (wp_store_offset with "arr↦"). 1: rewrite lookup_lt_is_Some...
     iNext. iIntros "[arr↦ arr👑]". iModIntro.
     iSplitL "t↦ b↦ arr↦ γ mta".
     { iNext. iExists t2, b, _. iFrame "t↦ b↦ arr↦".
-      rewrite slice_insert_right... iFrame. rewrite insert_length... }
+      rewrite slice_insert_right... iFrame. iPureIntro.
+      eapply (deque_bound_insert _ _ _ b)... }
     wp_pures.
     replace (Z.of_nat b + 1)%Z with (Z.of_nat (S b))...
 
     (* store bot *)
-    iInv "Inv" as (t3 b3 l3) ">(t↦ & b↦ & arr↦ & γ & mta & [%Htb3 %HL3])".
+    iInv "Inv" as (t3 b3 l3) ">(t↦ & b↦ & arr↦ & γ & mta & %BOUND3)".
       iDestruct (mapsto_agree with "b↦ b👑") as "%".
         injection H as [=]. apply Nat2Z.inj in H.
       iDestruct (array_agree with "arr↦ arr👑") as "%"; subst.
-        { rewrite insert_length... }
-      rewrite insert_length in HL3. clear t2 Htb2 HL2.
+        1: rewrite insert_length...
+      clear t2 BOUND2.
     iMod "AU" as (l') "[Cont [_ Commit]]".
       unfold deque_content.
       iDestruct (ghost_var_agree with "γ Cont") as "%"; subst.
@@ -219,15 +267,77 @@ Section proof.
     iDestruct "b↦" as "[b↦ b👑]".
     iMod (ghost_var_update_2 (slice (<[b:=v]> l) t3 (S b))
       with "γ Cont") as "[γ Cont]". { rewrite Qp.half_half... }
-    iMod (mono_toparr_append (slice (<[b:=v]> l) t3 b) [v] with "mta") as "mta".
+    iMod (mono_toparr_append _ (slice (<[b:=v]> l) t3 b) [v] with "mta") as "mta".
       rewrite <- slice_extend_right... 2: rewrite list_lookup_insert...
     iMod ("Commit" with "[Cont b👑 arr👑]") as "Φ".
-    { iFrame. iExists _,_,_,(S b),_; iFrame. repeat iSplit...
-      rewrite insert_length... }
+    { iFrame. iExists _,_,_,(S b),_; iFrame. iSplit... rewrite insert_length... }
     iModIntro. iModIntro.
     
     iFrame. unfold deque_inv. iNext. iExists _,_,_.
-    iFrame "t↦ b↦ arr↦ γ".
-    iSplit... rewrite insert_length...
+    iFrame "t↦ b↦ arr↦ γ". iSplit...
+    iPureIntro. apply deque_bound_extend_right...
   Qed.
+
+  Lemma steal_spec γq γt q :
+    is_deque γq γt q -∗
+    <<< ∀∀ l : list val, deque_content γq l >>>
+      steal q @ ↑N
+    <<< ∃∃ (l' : list val) (v : val),
+      deque_content γq l' ∗
+      match v with
+      | #() => ⌜l' = l⌝
+      | _ => ⌜l = [v] ++ l'⌝
+      end, RET v >>>.
+  Proof with autoall.
+    iIntros "#Is" (Φ) "AU".
+      iDestruct "Is" as (arr top bot) "[%Is Inv]". subst.
+    wp_lam. unfold code.arr, code.top, code.bot. wp_pures.
+
+    (* load top *)
+    wp_bind (! _)%E.
+    iInv "Inv" as (t1 b1 l1) ">(t↦ & b↦ & arr↦ & γ & mta & %BOUND1)".
+      iMod (mono_toparr_get_lb with "mta") as "[mta #mtlb1]".
+    wp_load.
+    iModIntro. iSplitL "t↦ b↦ arr↦ γ mta".
+      { iExists _,_,_. iFrame "t↦ b↦ arr↦ γ"... }
+    wp_pures.
+
+    (* load bot *)
+    wp_bind (! _)%E.
+    iInv "Inv" as (t2 b2 l2) ">(t↦ & b↦ & arr↦ & γ & mta & %BOUND2)".
+      iMod (mono_toparr_get_lb with "mta") as "[mta #mtlb2]".
+      iDestruct (mono_toparr_lb_own_top with "mta mtlb1") as "%Ht12".
+    wp_load.
+    iModIntro. iSplitL "t↦ b↦ arr↦ γ mta".
+      { iExists _,_,_. iFrame "t↦ b↦ arr↦ γ"... }
+    wp_pures.
+
+    (* no chance to steal *)
+    case_bool_decide; wp_pures.
+    { admit. }
+
+    (* cas top *)
+    wp_bind (CmpXchg _ _ _)%E.
+    iInv "Inv" as (t3 b3 l3) ">(t↦ & b↦ & arr↦ & γ & mta & %BOUND3)".
+      iDestruct (mono_toparr_lb_own_top with "mta mtlb2") as "%Ht23".
+    destruct (decide (t3 = t1)).
+    - (* success *)
+      assert (t1 = t2)... subst. wp_cmpxchg_suc.
+      assert (t2 < b3) by admit.
+      replace (Z.of_nat t2 + 1)%Z with (Z.of_nat (S t2))...
+      iMod (mono_toparr_top _ _ t2 (S t2) with "mta") as "mta"...
+      iMod "AU" as (l') "[Cont [_ Commit]]".
+        unfold deque_content.
+        iDestruct (ghost_var_agree with "γ Cont") as "%". subst.
+        iMod (ghost_var_update_2 (slice l3 (S t2) b3) with "γ Cont") as "[γ Cont]".
+          { rewrite Qp.half_half... }
+        assert (is_Some (l3 !! t2)) as [k HLk].
+          { rewrite lookup_lt_is_Some... }
+        iMod ("Commit" $! _ k with "[Cont]").
+          { iFrame. admit. }
+      iModIntro. iSplitL "t↦ b↦ arr↦ γ mta".
+        { iExists _,_,_. iFrame "t↦ b↦ arr↦ γ mta".
+          iNext. iPureIntro. apply deque_bound_shrink_left... }
+      wp_pures.
+  Admitted.
 End proof.
